formal/EFSM.thy
@@ -432,10 +432,12 @@ lemma prefix_closure: "accepts e s d (t@t') \<Longrightarrow> accepts e s d t"
 lemma accepts_head: "accepts e s d (h#t) \<Longrightarrow> accepts e s d [h]"
   using accepts_cons accepts.base by auto
 
-inductive gets_us_to :: "nat \<Rightarrow> transition_matrix \<Rightarrow> nat \<Rightarrow> registers \<Rightarrow> trace \<Rightarrow> bool" where
+inductive gets_us_to :: "cfstate \<Rightarrow> transition_matrix \<Rightarrow> cfstate \<Rightarrow> registers \<Rightarrow> trace \<Rightarrow> bool" where
   base: "s = target \<Longrightarrow> gets_us_to target _ s _ []" |
   step_some: "\<exists>(s', T) |\<in>| possible_steps e s d (fst h) (snd h). gets_us_to target e s' (apply_updates (Updates T) (join_ir i r) r) t \<Longrightarrow> gets_us_to target e s r (h#t)" |
   step_none: "step e s r (fst h) (snd h) = None \<Longrightarrow> s = target \<Longrightarrow> gets_us_to target e s r (h#t)"
+
+definition "trace_gets_us_to s e = gets_us_to s e 0 <>"
 
 lemma no_further_steps: "s \<noteq> s' \<Longrightarrow> \<not> gets_us_to s e s' r []"
   apply safe
