formal/inference/efsm2sal.thy
@@ -24,7 +24,7 @@ fun aexp2sal :: "aexp \<Rightarrow> String.literal" where
   "aexp2sal (L (Num n)) = STR ''Some(Num(''+ show_int n + STR ''))''"|
   "aexp2sal (L (value.Str n)) = STR ''Some(Str(String__''+ (if n = STR '''' then STR ''_EMPTY__'' else escape n replacements) + STR ''))''" |
   "aexp2sal (V (vname.I i)) = STR ''Some(i('' + show_nat (i+1) + STR ''))''" |
-  "aexp2sal (V (vname.R i)) = STR ''r('' + show_nat i + STR '')''" |
+  "aexp2sal (V (vname.R i)) = STR ''r__'' + show_nat i" |
   "aexp2sal (Plus a1 a2) = STR ''value_plus(''+aexp2sal a1 + STR '', '' + aexp2sal a2 + STR '')''" |
   "aexp2sal (Minus a1 a2) = STR ''value_minus(''+aexp2sal a1 + STR '', '' + aexp2sal a2 + STR '')''"
 
@@ -32,7 +32,7 @@ fun gexp2sal :: "gexp \<Rightarrow> String.literal" where
   "gexp2sal (Bc True) = STR ''True''" |
   "gexp2sal (Bc False) = STR ''False''" |
   "gexp2sal (Eq a1 a2) = STR ''gval(value_eq('' + aexp2sal a1 + STR '', '' + aexp2sal a2 + STR ''))''" |
-  "gexp2sal (Lt a1 a2) = STR ''gval(value_lt('' + aexp2sal a1 + STR '', '' + aexp2sal a2 + STR ''))''" |
+  "gexp2sal (Gt a1 a2) = STR ''gval(value_gt('' + aexp2sal a1 + STR '', '' + aexp2sal a2 + STR ''))''" |
   "gexp2sal (In v l) = join (map (\<lambda>l'.  STR ''gval(value_eq('' + aexp2sal (V v) + STR '', '' + aexp2sal (L l') + STR ''))'') l) STR '' OR ''" |
   "gexp2sal (Nor g1 g2) = STR ''NOT (gval('' + gexp2sal g1 + STR '') OR gval( '' + gexp2sal g2 + STR ''))''" |
   "gexp2sal (Null a1) = STR ''a1 = None''"
@@ -40,5 +40,27 @@ fun gexp2sal :: "gexp \<Rightarrow> String.literal" where
 fun guards2sal :: "gexp list \<Rightarrow> String.literal" where
   "guards2sal [] = STR ''TRUE''" |
   "guards2sal G = join (map gexp2sal G) STR '' AND ''"
+
+
+fun aexp2sal_num :: "aexp \<Rightarrow> nat \<Rightarrow> String.literal" where
+  "aexp2sal_num (L (Num n)) m = STR ''Some(Num(''+ show_int n + STR ''))''"|
+  "aexp2sal_num (L (value.Str n)) m = STR ''Some(Str(String__''+ (if n = STR '''' then STR ''_EMPTY__'' else escape n replacements) + STR ''))''" |
+  "aexp2sal_num (V (vname.I i)) m = STR ''Some(i('' + show_nat (i+1) + STR ''))''" |
+  "aexp2sal_num (V (vname.R i)) m = STR ''r__'' + show_nat i + STR ''.'' + show_nat m" |
+  "aexp2sal_num (Plus a1 a2) m = STR ''value_plus(''+aexp2sal a1 + STR '', '' + aexp2sal a2 + STR '')''" |
+  "aexp2sal_num (Minus a1 a2) m = STR ''value_minus(''+aexp2sal a1 + STR '', '' + aexp2sal a2 + STR '')''"
+
+fun gexp2sal_num :: "gexp \<Rightarrow> nat \<Rightarrow> String.literal" where
+  "gexp2sal_num (Bc True) m = STR ''True''" |
+  "gexp2sal_num (Bc False) m = STR ''False''" |
+  "gexp2sal_num (Eq a1 a2) m = STR ''gval(value_eq('' + aexp2sal_num a1 m + STR '', '' + aexp2sal_num a2 m + STR ''))''" |
+  "gexp2sal_num (Gt a1 a2) m = STR ''gval(value_gt('' + aexp2sal_num a1 m + STR '', '' + aexp2sal_num a2 m + STR ''))''" |
+  "gexp2sal_num (In v l) m = join (map (\<lambda>l'.  STR ''gval(value_eq('' + aexp2sal_num (V v) m + STR '', '' + aexp2sal_num (L l') m + STR ''))'') l) STR '' OR ''" |
+  "gexp2sal_num (Nor g1 g2) m = STR ''NOT (gval('' + gexp2sal_num g1 m + STR '') OR gval( '' + gexp2sal_num g2 m + STR ''))''" |
+  "gexp2sal_num (Null a1) m = STR ''a1 = None''"
+
+fun guards2sal_num :: "gexp list \<Rightarrow> nat \<Rightarrow> String.literal" where
+  "guards2sal_num [] _ = STR ''TRUE''" |
+  "guards2sal_num G m = join (map (\<lambda>g. gexp2sal_num g m) G) STR '' AND ''"
 
 end
